Switch to result monads in Dexter2 contract

examples/dexter2/Dexter2CPMM.v
@@ -14,6 +14,7 @@
 From ConCert.Utils Require Import RecordUpdate.
 From ConCert.Execution Require Import Blockchain.
 From ConCert.Execution Require Import Monads.
+From ConCert.Execution Require Import ResultMonad.
 From ConCert.Execution Require Import Serializable.
 From ConCert.Execution Require Import ContractCommon.
 From ConCert.Examples.FA2 Require Import FA2Token.
@@ -225,13 +226,15 @@ Module Dexter2 (SI : Dexter2Serializable) (NAddr : NullAddress).
     Definition amount_to_N : Amount -> N := Z.to_N.
     Definition N_to_amount : N -> Amount := Z.of_N.
 
-    Definition result : Type := option (State * list ActionBody).
-    Definition sub (n m : N) : option N := do _ <- throwIf (n <? m) ; Some (n - m).
-    Definition div (n m : N) : option N := do _ <- throwIf (m =? 0) ; Some (n / m).
-    Definition ceildiv (n m : N) : option N :=
+    Definition Result : Type := result (State * list ActionBody) unit.
+    Definition sub (n m : N) : result N unit :=
+      do _ <- throwIf (n <? m) tt; Ok (n - m).
+    Definition div (n m : N) : result N unit :=
+      do _ <- throwIf (m =? 0) tt; Ok (n / m).
+    Definition ceildiv (n m : N) : result N unit :=
       if N.modulo n m =? 0
       then div n m
-      else do result <- div n m ; Some (result + 1).
+      else do res <- div n m ; Ok (res + 1).
     Definition ceildiv_ (n m : N) : N :=
       if N.modulo n m =? 0
       then n / m
@@ -241,64 +244,83 @@ Module Dexter2 (SI : Dexter2Serializable) (NAddr : NullAddress).
     Opaque div.
     Opaque sub.
 
-    Definition non_zero_amount (amt : Z) : bool:= (0 <? amt)%Z.
+    Definition non_zero_amount (amt : Z) : bool := (0 <? amt)%Z.
     Global Arguments non_zero_amount _ /. (* always unfold, if applied *)
 
 
-    Definition call_liquidity_token (addr : Address) (amt : N) (msg : Dexter2FA12.Msg) :=
+    Definition call_liquidity_token (addr : Address)
+                                    (amt : N)
+                                    (msg : Dexter2FA12.Msg)
+                                    : ActionBody :=
       act_call addr (N_to_amount amt) (serialize msg).
 
     (** Note that [quantity] is allowed to be negative. In this case it correspons to burning *)
-    Definition mint_or_burn (state : State) (target : Address) (quantitiy : Z) : option ActionBody :=
-        do _ <- throwIf (address_eqb state.(lqtAddress) null_address) ; (* error lqtAddress not set *)
-        Some (call_liquidity_token state.(lqtAddress)
-                                  0
-                                  (Dexter2FA12.msg_mint_or_burn
-                                      (Dexter2FA12.build_mintOrBurn_param quantitiy target))).
+    Definition mint_or_burn (state : State)
+                            (target : Address)
+                            (quantitiy : Z)
+                            : result ActionBody unit :=
+        do _ <- throwIf (address_eqb state.(lqtAddress) null_address) tt; (* error lqtAddress not set *)
+        Ok (call_liquidity_token state.(lqtAddress)
+                      0
+                      (Dexter2FA12.msg_mint_or_burn
+                          (Dexter2FA12.build_mintOrBurn_param quantitiy target))).
 
-    Definition call_to_token (token_addr : Address) (amt : N) (msg : FA2Token.Msg) :=
+    Definition call_to_token (token_addr : Address)
+                             (amt : N)
+                             (msg : FA2Token.Msg) 
+                             : ActionBody :=
       act_call token_addr (N_to_amount amt) (serialize msg).
 
-    Definition token_transfer (state : State) (from to : Address) (amount : N) : ActionBody :=
+    Definition token_transfer (state : State)
+                              (from to : Address)
+                              (amount : N)
+                              : ActionBody :=
       call_to_token state.(tokenAddress)
-                    0
-                    (FA2Token.msg_transfer
-                      [FA2LegacyInterface.build_transfer from [FA2LegacyInterface.build_transfer_destination to state.(tokenId) amount] None]).
+                0
+                (FA2Token.msg_transfer
+                  [FA2LegacyInterface.build_transfer from 
+                  [FA2LegacyInterface.build_transfer_destination to state.(tokenId) amount] None]).
 
-    Definition xtz_transfer (to : Address) (amount : N) : option ActionBody :=
+    Definition xtz_transfer (to : Address)
+                            (amount : N)
+                            : result ActionBody unit :=
       if address_is_contract to
-      then None (* error_INVALID_TO_ADDRESS *)
-      else Some (act_transfer to (N_to_amount amount)).
+      then Err tt (* error_INVALID_TO_ADDRESS *)
+      else Ok (act_transfer to (N_to_amount amount)).
 
 
     (** ** Add liquidity *)
-    Definition add_liquidity (chain : Chain) (ctx : ContractCallContext)
-                            (state : State) (param : add_liquidity_param)
-                            : result :=
-      do _ <- throwIf state.(selfIsUpdatingTokenPool) ; (* error_SELF_IS_UPDATING_TOKEN_POOL_MUST_BE_FALSE *)
-      do _ <- throwIf (param.(add_deadline) <=? chain.(current_slot))%nat ; (* error_THE_CURRENT_TIME_MUST_BE_LESS_THAN_THE_DEADLINE *)
+    Definition add_liquidity (chain : Chain)
+                             (ctx : ContractCallContext)
+                             (state : State)
+                             (param : add_liquidity_param)
+                             : Result :=
+      do _ <- throwIf state.(selfIsUpdatingTokenPool) tt; (* error_SELF_IS_UPDATING_TOKEN_POOL_MUST_BE_FALSE *)
+      do _ <- throwIf (param.(add_deadline) <=? chain.(current_slot))%nat tt; (* error_THE_CURRENT_TIME_MUST_BE_LESS_THAN_THE_DEADLINE *)
       do lqt_minted <- div ((amount_to_N ctx.(ctx_amount)) * state.(lqtTotal)) state.(xtzPool) ; (* error_DIV_by_0 *)
       do tokens_deposited <- ceildiv ((amount_to_N ctx.(ctx_amount)) * state.(tokenPool)) state.(xtzPool) ; (* error_DIV_by_0 *)
-      do _ <- throwIf (param.(maxTokensDeposited) <? tokens_deposited) ; (* error_MAX_TOKENS_DEPOSITED_MUST_BE_GREATER_THAN_OR_EQUAL_TO_TOKENS_DEPOSITED *)
-      do _ <- throwIf (lqt_minted <? param.(minLqtMinted)) ; (* error_LQT_MINTED_MUST_BE_GREATER_THAN_MIN_LQT_MINTED *)
+      do _ <- throwIf (param.(maxTokensDeposited) <? tokens_deposited) tt; (* error_MAX_TOKENS_DEPOSITED_MUST_BE_GREATER_THAN_OR_EQUAL_TO_TOKENS_DEPOSITED *)
+      do _ <- throwIf (lqt_minted <? param.(minLqtMinted)) tt; (* error_LQT_MINTED_MUST_BE_GREATER_THAN_MIN_LQT_MINTED *)
       let new_state := state<| lqtTotal := state.(lqtTotal) + lqt_minted |>
                             <| tokenPool := state.(tokenPool) + tokens_deposited |>
                             <| xtzPool := state.(xtzPool) + (amount_to_N ctx.(ctx_amount))|> in
       let op_token := token_transfer state ctx.(ctx_from) ctx.(ctx_contract_address) tokens_deposited in
       do op_lqt <- mint_or_burn state param.(owner) (Z.of_N lqt_minted) ;
-      Some (new_state, [op_token; op_lqt]).
+      Ok (new_state, [op_token; op_lqt]).
 
     (** ** Remove liquidity *)
-    Definition remove_liquidity (chain : Chain) (ctx : ContractCallContext)
-                                (state : State) (param : remove_liquidity_param)
-                                : result :=
-      do _ <- throwIf state.(selfIsUpdatingTokenPool) ; (* error_SELF_IS_UPDATING_TOKEN_POOL_MUST_BE_FALSE *)
-      do _ <- throwIf (param.(remove_deadline) <=? chain.(current_slot))%nat ; (* error_THE_CURRENT_TIME_MUST_BE_LESS_THAN_THE_DEADLINE *)
-      do _ <- throwIf (non_zero_amount ctx.(ctx_amount)) ; (* error_AMOUNT_MUST_BE_ZERO *)
+    Definition remove_liquidity (chain : Chain)
+                                (ctx : ContractCallContext)
+                                (state : State)
+                                (param : remove_liquidity_param)
+                                : Result :=
+      do _ <- throwIf state.(selfIsUpdatingTokenPool) tt; (* error_SELF_IS_UPDATING_TOKEN_POOL_MUST_BE_FALSE *)
+      do _ <- throwIf (param.(remove_deadline) <=? chain.(current_slot))%nat tt; (* error_THE_CURRENT_TIME_MUST_BE_LESS_THAN_THE_DEADLINE *)
+      do _ <- throwIf (non_zero_amount ctx.(ctx_amount)) tt; (* error_AMOUNT_MUST_BE_ZERO *)
       do xtz_withdrawn <-  div (param.(lqtBurned) * state.(xtzPool)) state.(lqtTotal) ; (* error_DIV_by_0 *)
       do tokens_withdrawn <- div (param.(lqtBurned) * state.(tokenPool)) state.(lqtTotal) ; (* error_DIV_by_0 *)
-      do _ <- throwIf (xtz_withdrawn <? param.(minXtzWithdrawn)) ; (* error_THE_AMOUNT_OF_XTZ_WITHDRAWN_MUST_BE_GREATER_THAN_OR_EQUAL_TO_MIN_XTZ_WITHDRAWN *)
-      do _ <- throwIf (tokens_withdrawn <? param.(minTokensWithdrawn)) ; (* error_THE_AMOUNT_OF_TOKENS_WITHDRAWN_MUST_BE_GREATER_THAN_OR_EQUAL_TO_MIN_TOKENS_WITHDRAWN *)
+      do _ <- throwIf (xtz_withdrawn <? param.(minXtzWithdrawn))tt ; (* error_THE_AMOUNT_OF_XTZ_WITHDRAWN_MUST_BE_GREATER_THAN_OR_EQUAL_TO_MIN_XTZ_WITHDRAWN *)
+      do _ <- throwIf (tokens_withdrawn <? param.(minTokensWithdrawn)) tt; (* error_THE_AMOUNT_OF_TOKENS_WITHDRAWN_MUST_BE_GREATER_THAN_OR_EQUAL_TO_MIN_TOKENS_WITHDRAWN *)
       do new_lqtPool <- sub state.(lqtTotal) param.(lqtBurned) ; (* error_CANNOT_BURN_MORE_THAN_THE_TOTAL_AMOUNT_OF_LQT *)
       do new_tokenPool <- sub state.(tokenPool) tokens_withdrawn ; (* error_TOKEN_POOL_MINUS_TOKENS_WITHDRAWN_IS_NEGATIVE *)
       do new_xtzPool <- sub state.(xtzPool) xtz_withdrawn ; (* mutez subtraction run time error *)
@@ -315,117 +337,138 @@ Module Dexter2 (SI : Dexter2Serializable) (NAddr : NullAddress).
           tokenAddress := state.(tokenAddress);
           tokenId := state.(tokenId);
           lqtAddress := state.(lqtAddress) |} in
-      Some (new_state, [op_lqt; op_token; opt_xtz]).
+      Ok (new_state, [op_lqt; op_token; opt_xtz]).
 
     (** ** XTZ to tokens *)
-    Definition xtz_to_token (chain : Chain) (ctx : ContractCallContext)
-                            (state : State) (param : xtz_to_token_param)
-                            : result :=
-      do _ <- throwIf state.(selfIsUpdatingTokenPool) ; (* error_SELF_IS_UPDATING_TOKEN_POOL_MUST_BE_FALSE *)
-      do _ <- throwIf (param.(xtt_deadline) <=? chain.(current_slot))%nat ; (* error_THE_CURRENT_TIME_MUST_BE_LESS_THAN_THE_DEADLINE *)
+    Definition xtz_to_token (chain : Chain)
+                            (ctx : ContractCallContext)
+                            (state : State)
+                            (param : xtz_to_token_param)
+                            : Result :=
+      do _ <- throwIf state.(selfIsUpdatingTokenPool) tt; (* error_SELF_IS_UPDATING_TOKEN_POOL_MUST_BE_FALSE *)
+      do _ <- throwIf (param.(xtt_deadline) <=? chain.(current_slot))%nat tt; (* error_THE_CURRENT_TIME_MUST_BE_LESS_THAN_THE_DEADLINE *)
       do tokens_bought <- div
         ((amount_to_N ctx.(ctx_amount)) * 997 * state.(tokenPool))
           (state.(xtzPool) * 1000 + ((amount_to_N ctx.(ctx_amount)) * 997)) ; (* error_DIV_by_0 *)
-      do _ <- throwIf (tokens_bought <? param.(minTokensBought)) ; (* error_TOKENS_BOUGHT_MUST_BE_GREATER_THAN_OR_EQUAL_TO_MIN_TOKENS_BOUGHT *)
+      do _ <- throwIf (tokens_bought <? param.(minTokensBought)) tt; (* error_TOKENS_BOUGHT_MUST_BE_GREATER_THAN_OR_EQUAL_TO_MIN_TOKENS_BOUGHT *)
       do new_tokenPool <- sub state.(tokenPool) tokens_bought ; (* error_TOKEN_POOL_MINUS_TOKENS_BOUGHT_IS_NEGATIVE *)
       let new_state := state<| xtzPool := state.(xtzPool) + (amount_to_N ctx.(ctx_amount)) |>
                             <| tokenPool := new_tokenPool |> in
       let op := token_transfer state ctx.(ctx_contract_address) param.(tokens_to) tokens_bought in
-      Some (new_state, [op]).
+      Ok (new_state, [op]).
 
     (** ** Tokes to XTZ *)
-    Definition token_to_xtz (chain : Chain) (ctx : ContractCallContext)
-                            (state : State) (param : token_to_xtz_param)
-                            : result :=
-      do _ <- throwIf state.(selfIsUpdatingTokenPool) ; (* error_SELF_IS_UPDATING_TOKEN_POOL_MUST_BE_FALSE *)
-      do _ <- throwIf (param.(ttx_deadline) <=? chain.(current_slot))%nat ; (* error_THE_CURRENT_TIME_MUST_BE_LESS_THAN_THE_DEADLINE *)
-      do _ <- throwIf (non_zero_amount ctx.(ctx_amount)) ; (* error_AMOUNT_MUST_BE_ZERO *)
+    Definition token_to_xtz (chain : Chain)
+                            (ctx : ContractCallContext)
+                            (state : State)
+                            (param : token_to_xtz_param)
+                            : Result :=
+      do _ <- throwIf state.(selfIsUpdatingTokenPool) tt; (* error_SELF_IS_UPDATING_TOKEN_POOL_MUST_BE_FALSE *)
+      do _ <- throwIf (param.(ttx_deadline) <=? chain.(current_slot))%nat tt; (* error_THE_CURRENT_TIME_MUST_BE_LESS_THAN_THE_DEADLINE *)
+      do _ <- throwIf (non_zero_amount ctx.(ctx_amount)) tt; (* error_AMOUNT_MUST_BE_ZERO *)
       do xtz_bought <- div
         (param.(tokensSold) * 997 * state.(xtzPool))
           (state.(tokenPool) * 1000 + (param.(tokensSold) * 997)) ; (* error_DIV_by_0 *)
-      do _ <- throwIf (xtz_bought <? param.(minXtzBought)) ; (* error_XTZ_BOUGHT_MUST_BE_GREATER_THAN_OR_EQUAL_TO_MIN_XTZ_BOUGHT *)
+      do _ <- throwIf (xtz_bought <? param.(minXtzBought)) tt; (* error_XTZ_BOUGHT_MUST_BE_GREATER_THAN_OR_EQUAL_TO_MIN_XTZ_BOUGHT *)
       do new_xtzPool <- sub state.(xtzPool) xtz_bought ; (* mutez subtraction run time error *)
       let op_token := token_transfer state ctx.(ctx_from) ctx.(ctx_contract_address) param.(tokensSold) in
       do op_tez <- xtz_transfer param.(xtz_to) xtz_bought ;
       let new_state := state<| tokenPool := state.(tokenPool) + param.(tokensSold) |>
                             <| xtzPool := new_xtzPool |> in
-      Some (new_state, [op_token; op_tez]).
+      Ok (new_state, [op_token; op_tez]).
 
     (** ** Default entrypoint *)
-    Definition default_ (chain : Chain) (ctx : ContractCallContext)
-                        (state : State) : result :=
-      do _ <- throwIf state.(selfIsUpdatingTokenPool) ; (* error_SELF_IS_UPDATING_TOKEN_POOL_MUST_BE_FALSE *)
+    Definition default_ (chain : Chain)
+                        (ctx : ContractCallContext)
+                        (state : State)
+                        : Result :=
+      do _ <- throwIf state.(selfIsUpdatingTokenPool) tt; (* error_SELF_IS_UPDATING_TOKEN_POOL_MUST_BE_FALSE *)
       let new_state := state<| xtzPool := state.(xtzPool) + amount_to_N ctx.(ctx_amount) |> in
-        Some (new_state, []).
+        Ok (new_state, []).
 
     (** ** Set baker *)
-    Definition set_baker (chain : Chain) (ctx : ContractCallContext)
-                        (state : State) (param : set_baker_param)
-                        : result :=
-      do _ <- throwIf state.(selfIsUpdatingTokenPool) ; (* error_SELF_IS_UPDATING_TOKEN_POOL_MUST_BE_FALSE *)
-      do _ <- throwIf (non_zero_amount ctx.(ctx_amount)) ; (* error_AMOUNT_MUST_BE_ZERO *)
-      do _ <- throwIf (negb (address_eqb ctx.(ctx_from) state.(manager))) ; (* error_ONLY_MANAGER_CAN_SET_BAKER *)
-      do _ <- throwIf (state.(freezeBaker)) ; (* error_BAKER_PERMANENTLY_FROZEN *)
-        Some (state<| freezeBaker := param.(freezeBaker_) |>, set_delegate_call param.(baker)).
+    Definition set_baker (chain : Chain)
+                         (ctx : ContractCallContext)
+                         (state : State)
+                         (param : set_baker_param)
+                         : Result :=
+      do _ <- throwIf state.(selfIsUpdatingTokenPool) tt; (* error_SELF_IS_UPDATING_TOKEN_POOL_MUST_BE_FALSE *)
+      do _ <- throwIf (non_zero_amount ctx.(ctx_amount)) tt; (* error_AMOUNT_MUST_BE_ZERO *)
+      do _ <- throwIf (negb (address_eqb ctx.(ctx_from) state.(manager))) tt; (* error_ONLY_MANAGER_CAN_SET_BAKER *)
+      do _ <- throwIf (state.(freezeBaker)) tt; (* error_BAKER_PERMANENTLY_FROZEN *)
+        Ok (state<| freezeBaker := param.(freezeBaker_) |>, set_delegate_call param.(baker)).
 
     (** ** Set manager *)
-    Definition set_manager (chain : Chain) (ctx : ContractCallContext)
-                          (state : State) (new_manager : Address)
-                          : result :=
-      do _ <- throwIf state.(selfIsUpdatingTokenPool) ; (* error_SELF_IS_UPDATING_TOKEN_POOL_MUST_BE_FALSE *)
-      do _ <- throwIf (non_zero_amount ctx.(ctx_amount)) ; (* error_AMOUNT_MUST_BE_ZERO *)
-      do _ <- throwIf (negb (address_eqb ctx.(ctx_from) state.(manager))) ; (* error_ONLY_MANAGER_CAN_SET_MANAGER *)
-        Some (state<| manager := new_manager |>, []).
+    Definition set_manager (chain : Chain)
+                           (ctx : ContractCallContext)
+                           (state : State)
+                           (new_manager : Address)
+                           : Result :=
+      do _ <- throwIf state.(selfIsUpdatingTokenPool) tt; (* error_SELF_IS_UPDATING_TOKEN_POOL_MUST_BE_FALSE *)
+      do _ <- throwIf (non_zero_amount ctx.(ctx_amount)) tt; (* error_AMOUNT_MUST_BE_ZERO *)
+      do _ <- throwIf (negb (address_eqb ctx.(ctx_from) state.(manager))) tt; (* error_ONLY_MANAGER_CAN_SET_MANAGER *)
+        Ok (state<| manager := new_manager |>, []).
 
     (** ** Set liquidity address *)
-    Definition set_lqt_address (chain : Chain) (ctx : ContractCallContext)
-                              (state : State) (new_lqt_address : Address)
-                              : result :=
-      do _ <- throwIf state.(selfIsUpdatingTokenPool) ; (* error_SELF_IS_UPDATING_TOKEN_POOL_MUST_BE_FALSE *)
-      do _ <- throwIf (non_zero_amount ctx.(ctx_amount)) ; (* error_AMOUNT_MUST_BE_ZERO *)
-      do _ <- throwIf (negb (address_eqb ctx.(ctx_from) state.(manager))) ; (* error_ONLY_MANAGER_CAN_SET_LQT_ADRESS *)
-      do _ <- throwIf (negb (address_eqb state.(lqtAddress) null_address)) ; (* error_LQT_ADDRESS_ALREADY_SET *)
-        Some (state<| lqtAddress := new_lqt_address |>, []).
+    Definition set_lqt_address (chain : Chain)
+                               (ctx : ContractCallContext)
+                               (state : State)
+                               (new_lqt_address : Address)
+                               : Result :=
+      do _ <- throwIf state.(selfIsUpdatingTokenPool) tt; (* error_SELF_IS_UPDATING_TOKEN_POOL_MUST_BE_FALSE *)
+      do _ <- throwIf (non_zero_amount ctx.(ctx_amount)) tt; (* error_AMOUNT_MUST_BE_ZERO *)
+      do _ <- throwIf (negb (address_eqb ctx.(ctx_from) state.(manager))) tt; (* error_ONLY_MANAGER_CAN_SET_LQT_ADRESS *)
+      do _ <- throwIf (negb (address_eqb state.(lqtAddress) null_address)) tt; (* error_LQT_ADDRESS_ALREADY_SET *)
+        Ok (state<| lqtAddress := new_lqt_address |>, []).
 
     (** ** Update token pool *)
-    Definition update_token_pool (chain : Chain) (ctx : ContractCallContext)
-                                (state : State) : result :=
-      do _ <- throwIf (negb (address_eqb ctx.(ctx_from) ctx.(ctx_origin))) ; (* error_CALL_NOT_FROM_AN_IMPLICIT_ACCOUNT *)
-      do _ <- throwIf (non_zero_amount ctx.(ctx_amount)) ; (* error_AMOUNT_MUST_BE_ZERO *)
-      do _ <- throwIf state.(selfIsUpdatingTokenPool) ; (* error_UNEXPECTED_REENTRANCE_IN_UPDATE_TOKEN_POOL *)
+    Definition update_token_pool (chain : Chain)
+                                 (ctx : ContractCallContext)
+                                 (state : State)
+                                 : Result :=
+      do _ <- throwIf (negb (address_eqb ctx.(ctx_from) ctx.(ctx_origin))) tt; (* error_CALL_NOT_FROM_AN_IMPLICIT_ACCOUNT *)
+      do _ <- throwIf (non_zero_amount ctx.(ctx_amount)) tt; (* error_AMOUNT_MUST_BE_ZERO *)
+      do _ <- throwIf state.(selfIsUpdatingTokenPool) tt; (* error_UNEXPECTED_REENTRANCE_IN_UPDATE_TOKEN_POOL *)
       let balance_of_request :=
         FA2LegacyInterface.Build_balance_of_request ctx.(ctx_contract_address) state.(tokenId) in
       let balance_of_param :=
         FA2LegacyInterface.Build_balance_of_param [balance_of_request] (FA2LegacyInterface.Build_callback _ None ctx.(ctx_contract_address)) in
       let op := call_to_token state.(tokenAddress) 0 (FA2Token.msg_balance_of balance_of_param) in
-        Some (state<| selfIsUpdatingTokenPool := true |>, [op]).
+        Ok (state<| selfIsUpdatingTokenPool := true |>, [op]).
 
     (** ** Update token pool internal *)
-    Definition update_token_pool_internal (chain : Chain) (ctx : ContractCallContext)
-                                          (state : State) (token_pool : update_token_pool_internal_)
-                                          : result :=
+    Definition update_token_pool_internal (chain : Chain)
+                                          (ctx : ContractCallContext)
+                                          (state : State)
+                                          (token_pool : update_token_pool_internal_)
+                                          : Result :=
       do _ <- throwIf ((negb state.(selfIsUpdatingTokenPool)) ||
-                        (negb (address_eqb ctx.(ctx_from) state.(tokenAddress)))) ; (* error_THIS_ENTRYPOINT_MAY_ONLY_BE_CALLED_BY_GETBALANCE_OF_TOKENADDRESS *)
-      do _ <- throwIf (non_zero_amount ctx.(ctx_amount)) ; (* error_AMOUNT_MUST_BE_ZERO *)
+                        (negb (address_eqb ctx.(ctx_from) state.(tokenAddress)))) tt; (* error_THIS_ENTRYPOINT_MAY_ONLY_BE_CALLED_BY_GETBALANCE_OF_TOKENADDRESS *)
+      do _ <- throwIf (non_zero_amount ctx.(ctx_amount)) tt; (* error_AMOUNT_MUST_BE_ZERO *)
       do token_pool <-
         match token_pool with
-        | [] => None (* error_INVALID_FA2_BALANCE_RESPONSE *)
-        | x :: xs => Some x.(balance)
+        | [] => Err tt (* error_INVALID_FA2_BALANCE_RESPONSE *)
+        | x :: xs => Ok x.(balance)
         end ;
-      let new_state := state<| tokenPool := token_pool |><| selfIsUpdatingTokenPool := false |> in
-      Some (new_state, []).
+      let new_state := state<| tokenPool := token_pool |>
+                            <| selfIsUpdatingTokenPool := false |> in
+      Ok (new_state, []).
 
-    Definition call_to_other_token (token_addr : Address) (amount : N)
-              (msg : @FA2Token.FA2ReceiverMsg _ DexterMsg) :=
+    Definition call_to_other_token (token_addr : Address)
+                                   (amount : N)
+                                   (msg : @FA2Token.FA2ReceiverMsg _ DexterMsg)
+                                   : ActionBody :=
       act_call token_addr (N_to_amount amount) (serialize msg).
 
     (** ** Tokens to tokens *)
-    Definition token_to_token (chain : Chain) (ctx : ContractCallContext)
-                              (state : State) (param : token_to_token_param)
-                              : result :=
-      do _ <- throwIf state.(selfIsUpdatingTokenPool) ; (* error_SELF_IS_UPDATING_TOKEN_POOL_MUST_BE_FALSE *)
-      do _ <- throwIf (non_zero_amount ctx.(ctx_amount)) ; (* error_AMOUNT_MUST_BE_ZERO *)
-      do _ <- throwIf (param.(ttt_deadline) <=? chain.(current_slot))%nat ; (* error_THE_CURRENT_TIME_MUST_BE_LESS_THAN_THE_DEADLINE *)
+    Definition token_to_token (chain : Chain)
+                              (ctx : ContractCallContext)
+                              (state : State)
+                              (param : token_to_token_param)
+                              : Result :=
+      do _ <- throwIf state.(selfIsUpdatingTokenPool) tt; (* error_SELF_IS_UPDATING_TOKEN_POOL_MUST_BE_FALSE *)
+      do _ <- throwIf (non_zero_amount ctx.(ctx_amount)) tt; (* error_AMOUNT_MUST_BE_ZERO *)
+      do _ <- throwIf (param.(ttt_deadline) <=? chain.(current_slot))%nat tt; (* error_THE_CURRENT_TIME_MUST_BE_LESS_THAN_THE_DEADLINE *)
       do xtz_bought <- div
         (param.(tokensSold_) * 997 * state.(xtzPool))
           (state.(tokenPool) * 1000 + (param.(tokensSold_) * 997)) ; (* error_DIV_by_0 *)
@@ -441,14 +484,14 @@ Module Dexter2 (SI : Dexter2Serializable) (NAddr : NullAddress).
                                             minTokensBought := param.(minTokensBought_);
                                             xtt_deadline := param.(ttt_deadline)
                                           |})) in
-      Some (new_state, [op1; op2]).
+      Ok (new_state, [op1; op2]).
 
     (** ** Receive *)
     Definition receive_cpmm (chain : Chain)
                       (ctx : ContractCallContext)
                       (state : State)
                       (maybe_msg : option Msg)
-                      : result :=
+                      : Result :=
       match maybe_msg with
       | Some (FA2Token.other_msg (AddLiquidity param)) =>
           add_liquidity chain ctx state param
@@ -472,14 +515,15 @@ Module Dexter2 (SI : Dexter2Serializable) (NAddr : NullAddress).
           token_to_token chain ctx state param
       | Some (FA2Token.receive_balance_of_param responses) =>
           update_token_pool_internal chain ctx state responses
-      | _ => None
+      | _ => Err tt
       end.
 
     (** ** Init *)
     Definition init_cpmm (chain : Chain)
-                    (ctx : ContractCallContext)
-                    (setup : Setup) : option State :=
-      Some {|
+                         (ctx : ContractCallContext)
+                         (setup : Setup)
+                         : result State unit :=
+      Ok {|
         tokenPool := 0;
         xtzPool := 0;
         lqtTotal := setup.(lqtTotal_);
@@ -491,7 +535,7 @@ Module Dexter2 (SI : Dexter2Serializable) (NAddr : NullAddress).
         lqtAddress := null_address
       |}.
 
-    Definition contract : Contract Setup Msg State :=
+    Definition contract : Contract Setup Msg State unit :=
       build_contract init_cpmm receive_cpmm.
 
   End DexterDefs.
