examples/dexter2/Dexter2Extract.v
@@ -10,6 +10,7 @@ From ConCert.Extraction Require Import CameLIGOExtract.
 From ConCert.Execution Require Import Serializable.
 From ConCert.Execution Require Import Blockchain.
 From ConCert.Execution Require Import Containers.
+From ConCert.Execution Require Import ResultMonad.
 From ConCert.Execution Require ContractCommon.
 From ConCert.Examples.Dexter2 Require Dexter2CPMM.
 From ConCert.Examples.Dexter2 Require Dexter2FA12.
@@ -163,8 +164,8 @@ Module Dexter2LqtExtraction.
       there is no concept of initialisation function. However, it's common
       to provide a function that computes a valid initial storage that can
       be used for deployment. *)
-  Definition init (setup : Setup) : option State :=
-    Some {|
+  Definition init (setup : Setup) : result State unit :=
+    Ok {|
         tokens := ContractCommon.AddressMap.add setup.(lqt_provider) setup.(initial_pool) ContractCommon.AddressMap.empty;
         allowances := empty_allowance;
         admin := setup.(admin_);
@@ -181,16 +182,16 @@ Module Dexter2LqtExtraction.
        (ctx : ContractCallContext)
        (state : State)
        (maybe_msg : option Dexter2FA12.Msg)
-    : option (list ActionBody * State) :=
+    : result (list ActionBody * State) unit :=
     match DEX2LQTExtract.receive_lqt chain ctx state maybe_msg with
-    | Some x => Some (x.2, x.1)
-    | None => None
+    | Ok x => Ok (x.2, x.1)
+    | Err e => Err e
     end.
 
   Definition TT_remap_all :=
     (TT_remap_arith ++ TT_remap_dexter2 ++ TT_Dexter2_Lqt)%list.
 
-  Definition LIGO_DEXTER2LQT_MODULE : CameLIGOMod Msg ContractCallContext Setup State ActionBody :=
+  Definition LIGO_DEXTER2LQT_MODULE : CameLIGOMod Msg ContractCallContext Setup State ActionBody unit :=
   {| (* a name for the definition with the extracted code *)
      lmd_module_name := "cameLIGO_dexter2lqt" ;
 
@@ -280,8 +281,8 @@ Section D2E.
     (TT_remap_arith ++ TT_remap_dexter2 ++ TT_Dexter2_CPMM)%list.
 
   (** We redefine [init] for the same reasons as for the liquidity token *)
-  Definition init (setup : Setup) : option State :=
-    Some {|
+  Definition init (setup : Setup) : result State unit :=
+    Ok {|
         tokenPool := 0;
         xtzPool := 0;
         lqtTotal := setup.(lqtTotal_);
@@ -301,16 +302,16 @@ Section D2E.
 
 
   Definition receive_ (chain : Chain)
-       (ctx : ContractCallContext)
-       (state : State)
-       (maybe_msg : option Dexter2CPMM.Msg)
-    : option (list ActionBody * State) :=
+                      (ctx : ContractCallContext)
+                      (state : State)
+                      (maybe_msg : option Dexter2CPMM.Msg)
+                      : result (list ActionBody * State) unit :=
     match DEX2Extract.receive_cpmm chain ctx state maybe_msg with
-    | Some x => Some (x.2, x.1)
-    | None => None
+    | Ok x => Ok (x.2, x.1)
+    | Err e => Err e
     end.
 
-  Definition LIGO_DEXTER2_MODULE : CameLIGOMod Msg ContractCallContext Setup State ActionBody :=
+  Definition LIGO_DEXTER2_MODULE : CameLIGOMod Msg ContractCallContext Setup State ActionBody unit :=
   {| (* a name for the definition with the extracted code *)
      lmd_module_name := "cameLIGO_dexter2" ;
 
